update

src/ReplicatedDisk/ReplicatedDiskImpl.v
@@ -382,11 +382,17 @@ Module RD.
     Proof.
       unfold DiskSizeInit.
       step.
+      destruct r.
       step.
-      destruct r; descend; intuition eauto.
-      - destruct r; try step.
-        destruct (v == v0); step.
-      - destruct r; step.
+      - destruct r.
+        + destruct (size H0 == v).
+          * step.
+          * step.
+        + step.
+      - step.
+        destruct r.
+        + step.
+        + step.
     Qed.
 
     Hint Resolve DiskSizeInit_ok.
@@ -444,9 +450,527 @@ Module RD.
      * Recovery implementation.
      *)
 
+    Inductive RecStatus :=
+    (* continue working, nothing interesting has happened *)
+    | Continue
+    (* some address has been repaired (or the recovery has exhausted the
+       addresses) - only one address can be out of sync and thus only it must be
+       recovered. *)
+    (* OR, one of the disks has failed, so don't bother continuing recovery since
+       the invariant is now trivially satisfied *)
+    | RepairDoneOrFailed.
+
+    Definition fixup (a:addr) : prog RecStatus :=
+      mv0 <- Prim td (TD.Read d0 a);
+      match mv0 with
+      | Working v =>
+        mv2 <- Prim td (TD.Read d1 a);
+        match mv2 with
+        | Working v' =>
+          if v == v' then
+            Ret Continue
+          else
+            mu <- Prim td (TD.Write d1 a v);
+            Ret RepairDoneOrFailed
+        | Failed => Ret RepairDoneOrFailed
+        end
+      | Failed => Ret RepairDoneOrFailed
+      end.
+
+    (* recursively performs recovery at [a-1], [a-2], down to 0 *)
+    Fixpoint recover_at (a:addr) : prog unit :=
+      match a with
+      | 0 => Ret tt
+      | S n =>
+        s <- fixup n;
+        match s with
+        | Continue => recover_at n
+        | RepairDoneOrFailed => Ret tt
+        end
+      end.
 
     Definition Recover : prog unit :=
+      sz <- DiskSize;
+      _ <- recover_at sz;
       Ret tt.
+
+
+    (**
+     * Lemmas and recovery proofs.
+     *)
+
+    Lemma if_lt_dec : forall A n m (a a':A),
+        n < m ->
+        (if lt_dec n m then a else a') = a.
+    Proof.
+      intros.
+      destruct (lt_dec n m); auto.
+      contradiction.
+    Qed.
+
+    Lemma disks_eq_inbounds : forall T (d: diskOf T) a v v',
+        a < size d ->
+        d a ?|= eq v ->
+        d a ?|= eq v' ->
+        v = v'.
+    Proof.
+      unfold disk_get; intros.
+      pose proof (diskMem_domain d a).
+      rewrite if_lt_dec in H2 by auto.
+      repeat deex.
+      rewrite H2 in H0.
+      replace (d a) in *; simpl in *; subst; auto.
+    Qed.
+
+    (* we will show that fixup does nothing once the disks are the same *)
+    Theorem fixup_equal_ok : forall a,
+        prog_spec
+          (fun d state =>
+             {|
+               pre :=
+                 (* for simplicity we only consider in-bounds addresses, though
+                    if a is out-of-bounds fixup just might uselessly write to
+                    disk and not do anything *)
+                 a < size d /\
+                 TD.disk0 state ?|= eq d /\
+                 TD.disk1 state ?|= eq d;
+               post :=
+                 fun r state' =>
+                   match r with
+                   | Continue =>
+                     TD.disk0 state' ?|= eq d /\
+                     TD.disk1 state' ?|= eq d
+                   | RepairDoneOrFailed =>
+                     TD.disk0 state' ?|= eq d /\
+                     TD.disk1 state' ?|= eq d
+                   end;
+               recover :=
+                 fun _ state' =>
+                   TD.disk0 state' ?|= eq d /\
+                   TD.disk1 state' ?|= eq d;
+             |})
+          (fixup a)
+          (irec td)
+          (interface_abs td).
+    Proof.
+      unfold fixup.
+      step.
+
+      destruct r; step.
+
+      destruct r; try step.
+      is_eq v v0; try step.
+      assert (v = v0) by eauto using disks_eq_inbounds.
+      contradiction.
+    Qed.
+
+    Lemma diskUpd_maybe_same : forall (d:disk) a b,
+        d a ?|= eq b ->
+        diskUpd d a b = d.
+    Proof.
+      intros.
+      destruct (d a) eqn:?; simpl in *; subst;
+        autorewrite with upd;
+        auto.
+    Qed.
+
+    Hint Rewrite diskUpd_maybe_same using (solve [ auto ]) : rd.
+    Hint Rewrite diskUpd_eq using (solve [ auto ]) : rd.
+
+    Theorem fixup_correct_addr_ok : forall a,
+        prog_spec
+          (fun '(d, b) state =>
+             {|
+               pre :=
+                 a < size d /\
+                 TD.disk0 state ?|= eq (diskUpd d a b) /\
+                 TD.disk1 state ?|= eq d;
+               post :=
+                 fun r state' =>
+                   match r with
+                   | Continue =>
+                     (* could happen if b already happened to be value *)
+                     TD.disk0 state' ?|= eq (diskUpd d a b) /\
+                     TD.disk1 state' ?|= eq (diskUpd d a b)
+                   | RepairDoneOrFailed =>
+                     TD.disk0 state' ?|= eq (diskUpd d a b) /\
+                     TD.disk1 state' ?|= eq (diskUpd d a b) \/
+                     TD.disk0 state' ?|= eq d /\
+                     TD.disk1 state' ?|= eq d
+                   end;
+               recover :=
+                 fun _ state' =>
+                   (TD.disk0 state' ?|= eq (diskUpd d a b) /\
+                    TD.disk1 state' ?|= eq (diskUpd d a b)) \/
+                   (TD.disk0 state' ?|= eq (diskUpd d a b) /\
+                    TD.disk1 state' ?|= eq d) \/
+                   (TD.disk0 state' ?|= eq d /\
+                    TD.disk1 state' ?|= eq d);
+             |})
+          (fixup a)
+          (irec td)
+          (interface_abs td).
+    Proof.
+      unfold fixup; intros.
+      step.
+
+      destruct r; try step.
+
+      destruct r; try step.
+      match goal with
+      | |- context[diskUpd _ _ ?b] =>
+        is_eq b v; try step
+      end.
+
+      step.
+      destruct r; (intuition eauto); simplify; finish.
+    Qed.
+
+    Hint Resolve PeanoNat.Nat.lt_neq.
+    Hint Rewrite diskUpd_neq : rd.
+    Hint Resolve disks_eq_inbounds.
+
+    Theorem fixup_wrong_addr_ok : forall a,
+        prog_spec
+          (fun '(d, b, a') state =>
+             {|
+               pre :=
+                 a < size d /\
+                 (* recovery, working from end of disk, has not yet reached the
+                    correct address *)
+                 a' < a /\
+                 TD.disk0 state ?|= eq (diskUpd d a' b) /\
+                 TD.disk1 state ?|= eq d;
+               post :=
+                 fun r state' =>
+                   match r with
+                   | Continue =>
+                     TD.disk0 state' ?|= eq (diskUpd d a' b) /\
+                     TD.disk1 state' ?|= eq d
+                   | RepairDoneOrFailed =>
+                     TD.disk0 state' ?|= eq d /\
+                     TD.disk1 state' ?|= eq d \/
+                     TD.disk0 state' ?|= eq (diskUpd d a' b) /\
+                     TD.disk1 state' ?|= eq (diskUpd d a' b)
+                   end;
+               recover :=
+                 fun _ state' =>
+                   (TD.disk0 state' ?|= eq (diskUpd d a' b) /\
+                    TD.disk1 state' ?|= eq d) \/
+                   (TD.disk0 state' ?|= eq d /\
+                    TD.disk1 state' ?|= eq d);
+             |})
+          (fixup a)
+          (irec td)
+          (interface_abs td).
+    Proof.
+      unfold fixup; intros.
+      step.
+
+      destruct r; try step.
+
+      destruct r; try step.
+      is_eq v v0; try step.
+    Qed.
+
+    (* To make these specifications precise while also covering both the already
+     * synced and diverged disks cases, we keep track of which input state we're
+     * in from the input and use it to give an exact postcondition. *)
+    Inductive DiskStatus :=
+    | FullySynced
+    | OutOfSync (a:addr) (b:block).
+
+    Theorem fixup_ok : forall a,
+        prog_spec
+          (fun '(d, s) state =>
+             {|
+               pre :=
+                 a < size d /\
+                 match s with
+                 | FullySynced => TD.disk0 state ?|= eq d /\
+                                 TD.disk1 state ?|= eq d
+                 | OutOfSync a' b => a' <= a /\
+                                    TD.disk0 state ?|= eq (diskUpd d a' b) /\
+                                    TD.disk1 state ?|= eq d
+                 end;
+               post :=
+                 fun r state' =>
+                   match s with
+                   | FullySynced => TD.disk0 state' ?|= eq d /\
+                                   TD.disk1 state' ?|= eq d
+                   | OutOfSync a' b =>
+                     match r with
+                     | Continue =>
+                       (a' < a /\
+                        TD.disk0 state' ?|= eq (diskUpd d a' b) /\
+                        TD.disk1 state' ?|= eq d) \/
+                       (TD.disk0 state' ?|= eq (diskUpd d a' b) /\
+                        TD.disk1 state' ?|= eq (diskUpd d a' b))
+                     | RepairDone =>
+                       (TD.disk0 state' ?|= eq d /\
+                        TD.disk1 state' ?|= eq d) \/
+                       (TD.disk0 state' ?|= eq (diskUpd d a' b) /\
+                        TD.disk1 state' ?|= eq (diskUpd d a' b))
+                     end
+                   end;
+               recover :=
+                 fun _ state' =>
+                   match s with
+                   | FullySynced => TD.disk0 state' ?|= eq d /\
+                                   TD.disk1 state' ?|= eq d
+                   | OutOfSync a' b =>
+                     (TD.disk0 state' ?|= eq (diskUpd d a' b) /\
+                      TD.disk1 state' ?|= eq (diskUpd d a' b)) \/
+                     (TD.disk0 state' ?|= eq (diskUpd d a' b) /\
+                      TD.disk1 state' ?|= eq d) \/
+                     (TD.disk0 state' ?|= eq d /\
+                      TD.disk1 state' ?|= eq d)
+                   end;
+             |})
+          (fixup a)
+          (irec td)
+          (interface_abs td).
+    Proof.
+      spec_cases; simplify.
+      match goal with | x : DiskStatus |- _ => rename x into s end.
+      destruct s; intuition eauto.
+      - spec_case fixup_equal_ok; simplify; finish.
+        descend; (intuition eauto); destruct matches in *;
+          intuition eauto.
+      - apply PeanoNat.Nat.lt_eq_cases in H1; intuition.
+        + spec_case fixup_wrong_addr_ok; simplify; finish.
+          descend; intuition eauto.
+
+          destruct v; intuition eauto.
+        + spec_case fixup_correct_addr_ok; simplify; finish.
+          descend; intuition eauto.
+
+          destruct v; intuition eauto.
+    Qed.
+
+    Hint Resolve fixup_ok.
+
+    Hint Resolve Lt.lt_n_Sm_le.
+
+    Hint Rewrite diskUpd_size : rd.
+
+    Theorem recover_at_ok : forall a,
+        prog_spec
+          (fun '(d, s) state =>
+             {|
+               pre :=
+                 a <= size d /\
+                 match s with
+                 | FullySynced => TD.disk0 state ?|= eq d /\
+                                 TD.disk1 state ?|= eq d
+                 | OutOfSync a' b => a' < a /\
+                                    TD.disk0 state ?|= eq (diskUpd d a' b) /\
+                                    TD.disk1 state ?|= eq d
+                 end;
+               post :=
+                 fun r state' =>
+                   match s with
+                   | FullySynced =>
+                     TD.disk0 state' ?|= eq d /\
+                     TD.disk1 state' ?|= eq d
+                   | OutOfSync a' b =>
+                     (TD.disk0 state' ?|= eq d /\
+                      TD.disk1 state' ?|= eq d) \/
+                     (TD.disk0 state' ?|= eq (diskUpd d a' b) /\
+                      TD.disk1 state' ?|= eq (diskUpd d a' b))
+                   end;
+               recover :=
+                 fun _ state' =>
+                   match s with
+                   | FullySynced => TD.disk0 state' ?|= eq d /\
+                                   TD.disk1 state' ?|= eq d
+                   | OutOfSync a' b =>
+                     (TD.disk0 state' ?|= eq d /\
+                      TD.disk1 state' ?|= eq d) \/
+                     (TD.disk0 state' ?|= eq (diskUpd d a' b) /\
+                      TD.disk1 state' ?|= eq d) \/
+                     (TD.disk0 state' ?|= eq (diskUpd d a' b) /\
+                      TD.disk1 state' ?|= eq (diskUpd d a' b))
+                   end;
+             |})
+          (recover_at a)
+          (irec td)
+          (interface_abs td).
+    Proof.
+      induction a; simpl; intros.
+      - step.
+        rename_by_type DiskStatus s.
+        destruct s; intuition (subst; eauto).
+        omega.
+      - step.
+        rename_by_type DiskStatus s.
+        destruct s; intuition (subst; eauto).
+        rename_by_type (diskOf block) d.
+        exists d, FullySynced; intuition eauto.
+        destruct r; step.
+
+        exists d, FullySynced; intuition eauto.
+        rename_by_type (diskOf block) d.
+        exists d, (OutOfSync a0 b); intuition eauto.
+
+        destruct r; step.
+        intuition.
+        exists d, (OutOfSync a0 b); intuition eauto.
+        exists (diskUpd d a0 b), FullySynced; intuition eauto.
+        simplify; finish.
+    Qed.
+
+    Hint Resolve recover_at_ok.
+
+    Definition Recover_spec :=
+      (fun '(d, s) state =>
+         {|
+           pre :=
+             match s with
+             | FullySynced => TD.disk0 state ?|= eq d /\
+                             TD.disk1 state ?|= eq d
+             | OutOfSync a b => a < size d /\
+                               TD.disk0 state ?|= eq (diskUpd d a b) /\
+                               TD.disk1 state ?|= eq d
+             end;
+           post :=
+             fun (_:unit) state' =>
+               match s with
+               | FullySynced => TD.disk0 state' ?|= eq d /\
+                               TD.disk1 state' ?|= eq d
+               | OutOfSync a b =>
+                 (TD.disk0 state' ?|= eq d /\
+                  TD.disk1 state' ?|= eq d) \/
+                 (TD.disk0 state' ?|= eq (diskUpd d a b) /\
+                  TD.disk1 state' ?|= eq (diskUpd d a b))
+               end;
+           recover :=
+             fun (_:unit) state' =>
+               match s with
+               | FullySynced => TD.disk0 state' ?|= eq d /\
+                               TD.disk1 state' ?|= eq d
+               | OutOfSync a b =>
+                 (TD.disk0 state' ?|= eq d /\
+                  TD.disk1 state' ?|= eq d) \/
+                 (TD.disk0 state' ?|= eq (diskUpd d a b) /\
+                  TD.disk1 state' ?|= eq d) \/
+                 (TD.disk0 state' ?|= eq (diskUpd d a b) /\
+                  TD.disk1 state' ?|= eq (diskUpd d a b))
+               end;
+         |}).
+
+    Theorem Recover_rok :
+      prog_spec
+        Recover_spec
+        (Recover)
+        (irec td)
+        (interface_abs td).
+    Proof.
+      (* Prove that [Recover] satisfies its spec above, [Recover_spec],
+       * in the absence of repeated recovery.
+       *)
+      pocs_admit.
+    Qed.
+
+    Theorem Recover_ok :
+      prog_loopspec
+        Recover_spec
+        (Recover)
+        (irec td)
+        (interface_abs td).
+    Proof.
+      (* Prove that [Recover] is safe to repeatedly crash and recover.
+       *)
+      eapply idempotent_loopspec; simpl.
+      - eapply Recover_rok.
+        pocs_admit.
+    Qed.
+
+    Hint Resolve Recover_ok.
+
+
+    (**
+     * Specifications and proofs about our implementation of the API
+     * with our own full recovery.
+     *)
+
+    Theorem Read_rok : forall a,
+        prog_spec
+          (fun d state =>
+             {|
+               pre := TD.disk0 state ?|= eq d /\
+                      TD.disk1 state ?|= eq d;
+               post :=
+                 fun r state' =>
+                   d a ?|= eq r /\
+                   TD.disk0 state' ?|= eq d /\
+                   TD.disk1 state' ?|= eq d;
+               recover :=
+                 fun _ state' =>
+                   TD.disk0 state' ?|= eq d /\
+                   TD.disk1 state' ?|= eq d;
+             |})
+          (Read a) (_ <- irec td; Recover)
+          (interface_abs td).
+    Proof.
+      start.
+      rename a0 into d.
+      descend; (intuition eauto); simplify.
+      exists d, FullySynced; intuition eauto.
+    Qed.
+
+    Theorem Write_rok : forall a b,
+        prog_spec
+          (fun d state =>
+             {|
+               pre :=
+                 TD.disk0 state ?|= eq d /\
+                 TD.disk1 state ?|= eq d;
+               post :=
+                 fun r state' =>
+                   r = tt /\
+                   TD.disk0 state' ?|= eq (diskUpd d a b) /\
+                   TD.disk1 state' ?|= eq (diskUpd d a b);
+               recover :=
+                 fun _ state' =>
+                    (TD.disk0 state' ?|= eq d /\
+                    TD.disk1 state' ?|= eq d) \/
+                   (TD.disk0 state' ?|= eq (diskUpd d a b) /\
+                    TD.disk1 state' ?|= eq (diskUpd d a b));
+              |})
+          (Write a b) (_ <- irec td; Recover)
+          (interface_abs td).
+    Proof.
+      (* Prove that [Recover] properly recovers from all crashes in [Write]. *)
+      pocs_admit.
+     Qed.
+
+    Theorem DiskSize_rok :
+      prog_spec
+        (fun d state =>
+           {|
+             pre := TD.disk0 state ?|= eq d /\
+                    TD.disk1 state ?|= eq d;
+             post :=
+               fun r state' =>
+                 r = size d /\
+                 TD.disk0 state' ?|= eq d /\
+                 TD.disk1 state' ?|= eq d;
+             recover :=
+               fun _ state' =>
+                 TD.disk0 state' ?|= eq d /\
+                 TD.disk1 state' ?|= eq d;
+           |})
+        (DiskSize) (_ <- irec td; Recover)
+        (interface_abs td).
+    Proof.
+      start.
+      rename a into d.
+      exists d, d; (intuition eauto); simplify.
+      exists d, FullySynced; intuition eauto.
+    Qed.
+
+    Hint Resolve Read_rok Write_rok DiskSize_rok Recover_rok.
 
 
     (* Now we gather up the implementation and all the correctness proofs,
